Energy is conserved
E<sub>tot</sub> = KE + PE 1/2mv<sup>2</sup> + 1/2kx<sup>2</sup>
=constant = initial energy

E = 1/2 K A<sup>2</sup>

You will always have SHM whenever the force is
1) restoring back to an equilibrium position
2) proportional to the distance from equilibrium
	F<sub>SHM</sub> = -constant (x - x<sub>equil</sub>)

This force always gives a = -ω<sup>2</sup> x, with solutions x(t) = A cos(ωt + Φ<sub>0</sub>)
For a mass-spring system where the force is given by Hooke's law
	F = ma = -k x , so a = -(k/m)x = -ω<sup>2</sup> x and ω = $\sqrt{k/m}$ 
	Note that k = - dF / dx

For other systems, the dependence of the force on displacement can be different and this leads to different expressions for ω
	But you can find effective spring constant from k = - dF / dx and still use ω = $\sqrt{k/m}$

General approach for finding ω
Find F<sub>Net</sub> = ΣF as a function of position x
Find equilibrium position x<sub>equil</sub> by solving F<sub>net</sub>(x<sub>equil</sub>) = 0
Solve for effective spring constant at x = x<sub>eq</sub> : k = - dF<sub>net</sub>(x<sub>equil</sub>) / dx
	ω = $\sqrt{k/m}$

F<sub>buoyant</sub> : magnitude is weight of liquid displaced

| F<sub>buoyant</sub> | = V<sub>D</sub> Ρ<sub>liquid</sub> g 

V<sub>D</sub> = volume of liquid displaced
P = density of liquid
g = gravity


[[PHYS 157 Lecture 28]]